Simplify the way that HeapFMap.v is refined

src/ByteStringFMap.v
@@ -30,10 +30,14 @@ Module Import HF := HeapFMap M.
 
 Import Within.
 Import Within.Block.
+Import Within.Block.FunMaps.
 
 Section Refined.
 
-Variable heap : Rep HSpec.
+Variable heap  : Rep HSpec.
+Variable heap' : ComputationalADT.cRep (projT1 HeapImpl).
+
+Variable heap_AbsR : Heap_AbsR (` heap) heap'.
 
 (* This style of computational refinement makes use of a separately refined
    heap. Another approach is to refine the heap methods directly, which would
@@ -41,7 +45,7 @@ Variable heap : Rep HSpec.
    proof word that is done in HeapFMap.v). *)
 
 Record PS' := {
-  ps'Heap : Rep HeapSpec;
+  ps'Heap : ComputationalADT.cRep (projT1 HeapImpl);
 
   ps'Buffer : N;
   ps'BufLen : N;
@@ -50,6 +54,7 @@ Record PS' := {
   ps'Length : N
 }.
 
+(*
 (* Strip away the proofy bits. *)
 Lemma ByteStringStrip :
   { adt : _ & refineADT (projT1 (ByteStringHeap heap)) adt }.
@@ -57,6 +62,216 @@ Proof.
   eexists.
   hone representation using
        (fun (or : PS) (nr : PS') =>
+          Heap_AbsR (` (psHeap or)) (ps'Heap nr) /\
+          psBuffer or = ps'Buffer nr /\
+          psBufLen or = ps'BufLen nr /\
+          psOffset or = ps'Offset nr /\
+          psLength or = ps'Length nr);
+  try simplify with monad laws; simpl.
+  {
+    refine pick val {| ps'Heap   := heap'
+                     ; ps'Buffer := 0
+                     ; ps'BufLen := 0
+                     ; ps'Offset := 0
+                     ; ps'Length := 0 |}.
+      finish honing.
+    simpl; intuition.
+  }
+  {
+    repeat match goal with
+      [ H : _ /\ _ |- _ ] => destruct H
+    end; subst.
+    destruct r_o, psHeap; simpl in *.
+    rewrite H1, H2, H3, H4.
+    rewrite refineEquiv_If_Then_Else_Bind.
+    apply refine_If_Then_Else.
+      simplify with monad laws; simpl.
+      unfold poke'; simpl.
+      remove_dependency; simpl.
+      erewrite Heap_refine_poke; eauto.
+      simplify with monad laws; simpl.
+      remember (M.mapi _ _) as M.
+      refine pick val {| ps'Heap   := (fst (ps'Heap r_n), M)
+                       ; ps'Buffer := ps'Buffer r_n
+                       ; ps'BufLen := ps'BufLen r_n
+                       ; ps'Offset := ps'Offset r_n - 1
+                       ; ps'Length := ps'Length r_n + 1 |};
+      rewrite HeqM; clear HeqM; simpl.
+        simplify with monad laws.
+        finish honing.
+      intuition.
+      apply of_map_Heap_AbsR.
+      admit.
+    rewrite refineEquiv_If_Then_Else_Bind.
+    subst H.
+    apply refine_If_Then_Else.
+      simplify with monad laws; simpl.
+      unfold memcpy', poke'; simpl.
+      remove_dependency; simpl.
+      setoid_rewrite refine_bind_dep_bind_ret; simpl.
+      do 2 setoid_rewrite refine_bind_dep_ignore.
+      erewrite Heap_refine_memcpy; eauto.
+      unfold wrap, FMap_memcpy.
+      rewrite refine_bind_unit.
+      {
+        erewrite Heap_refine_poke; eauto; simpl.
+        - simplify with monad laws; simpl.
+          remember (M.mapi _ _) as M.
+          refine pick val {| ps'Heap   := (fst (ps'Heap r_n), M)
+                           ; ps'Buffer := ps'Buffer r_n
+                           ; ps'BufLen := ps'BufLen r_n
+                           ; ps'Offset := 0
+                           ; ps'Length := ps'Length r_n + 1 |};
+          rewrite HeqM; clear HeqM; simpl.
+            simplify with monad laws.
+            finish honing.
+          intuition.
+          apply of_map_Heap_AbsR.
+          admit.
+        - apply of_map_Heap_AbsR.
+          admit.
+        - admit.
+      }
+    rewrite refineEquiv_If_Then_Else_Bind.
+    apply refine_If_Then_Else.
+      simplify with monad laws; simpl.
+      unfold alloc', memcpy', poke'.
+      remove_dependency; simpl.
+      do 3 setoid_rewrite refine_bind_dep_bind_ret.
+      simpl; remove_dependency.
+      do 3 setoid_rewrite refine_bind_dep_ignore.
+      unfold ByteStringHeap.buffer_cons_obligation_2.
+      etransitivity.
+        apply refine_under_bind; intros.
+        etransitivity.
+          apply refine_under_bind; intros.
+          etransitivity.
+            apply refine_under_bind; intros.
+            {
+              erewrite Heap_refine_poke; eauto.
+              - simplify with monad laws; simpl.
+                remember (M.mapi _ _) as M.
+                refine pick val {| ps'Heap   := (fst (ps'Heap r_n), M)
+                                 ; ps'Buffer := fst (ps'Heap r_n)
+                                 ; ps'BufLen := ps'Length r_n +1
+                                 ; ps'Offset := 0
+                                 ; ps'Length := ps'Length r_n + 1 |};
+                rewrite HeqM; clear HeqM; simpl.
+                  simplify with monad laws; simpl.
+                  finish honing.
+                intuition.
+                  apply of_map_Heap_AbsR.
+                  admit.
+                admit.
+              - 
+                unfold alloc in H. simpl in *.
+                destruct_computations; simpl in *.
+                eapply free_fromADT.
+                eapply memcpy_fromADT.
+                exact f.
+            etransitivity.
+              apply refine_under_bind; intros.
+      erewrite Heap_refine_alloc; eauto.
+      unfold wrap, FMap_alloc.
+      rewrite refine_bind_unit; simpl.
+      erewrite Heap_refine_memcpy; eauto.
+        Focus 3.
+        apply of_map_Heap_AbsR.
+        
+        apply for_all_add_true; eauto.
+      unfold wrap, FMap_memcpy.
+      rewrite refine_bind_unit; simpl.
+      erewrite Heap_refine_free; eauto.
+      unfold wrap, FMap_free.
+      rewrite refine_bind_unit; simpl.
+      erewrite Heap_refine_poke; eauto.
+      unfold wrap, FMap_poke.
+      rewrite refine_bind_unit; simpl.
+      remember (M.mapi _ _) as M.
+      refine pick val {| ps'Heap   := (fst (ps'Heap r_n), M)
+                       ; ps'Buffer := fst (ps'Heap r_n)
+                       ; ps'BufLen := ps'Length r_n +1
+                       ; ps'Offset := 0
+                       ; ps'Length := ps'Length r_n + 1 |};
+      rewrite HeqM; clear HeqM; simpl.
+        simplify with monad laws.
+        finish honing.
+      intuition.
+      admit.
+      admit.
+      admit.
+      admit.
+      admit.
+      admit.
+      admit.
+      admit.
+    unfold allocate_buffer, alloc', poke'.
+    simplify with monad laws; simpl.
+    remove_dependency; simpl.
+    setoid_rewrite refine_bind_dep_ret.
+    autorewrite with monad laws; simpl.
+    remove_dependency.
+    unfold ByteStringHeap.buffer_cons_obligation_3.
+    etransitivity.
+      apply refine_under_bind; intros.
+      remember (Map _ _) as M.
+      refine pick val {| ps'Heap   := M
+                       ; ps'Buffer := snd a
+                       ; ps'BufLen := 1
+                       ; ps'Offset := 0
+                       ; ps'Length := 1 |}.
+        simplify with monad laws.
+        rewrite HeqM.
+        finish honing.
+      intuition.
+    unfold alloc; simpl.
+    rewrite H0.
+    finish honing.
+  }
+  {
+    repeat match goal with
+      [ H : _ /\ _ |- _ ] => destruct H
+    end; subst.
+    rewrite H1, H2, H3, H4.
+    rewrite refineEquiv_If_Then_Else_Bind.
+    subst H.
+    apply refine_If_Then_Else.
+      simplify with monad laws; simpl.
+      unfold peek'.
+      remove_dependency.
+      rewrite H0.
+      etransitivity.
+        apply refine_under_bind; intros.
+        refine pick val {| ps'Heap   := ps'Heap r_n
+                         ; ps'Buffer := ps'Buffer r_n
+                         ; ps'BufLen := ps'BufLen r_n
+                         ; ps'Offset := if ps'Length r_n =? 1
+                                        then 0
+                                        else ps'Offset r_n + 1
+                         ; ps'Length := ps'Length r_n - 1 |}.
+          simplify with monad laws.
+          finish honing.
+        intuition.
+      simpl.
+      finish honing.
+    simplify with monad laws; simpl.
+    rewrite H0.
+    refine pick val r_n.
+      simplify with monad laws; simpl.
+      finish honing.
+    intuition.
+  }
+  apply reflexivityT.
+Defined.
+
+(* Strip away the proofy bits. *)
+Lemma ByteStringStrip :
+  { adt : _ & refineADT (projT1 (ByteStringHeap heap)) adt }.
+Proof.
+  eexists.
+  hone representation using
+       (fun (or : PS) (nr : PS') =>
+          (* Same (` (psHeap or)) (ps'Heap nr) /\ *)
           ` (psHeap or) = ps'Heap nr /\
           psBuffer or = ps'Buffer nr /\
           psBufLen or = ps'BufLen nr /\
@@ -76,13 +291,13 @@ Proof.
     repeat match goal with
       [ H : _ /\ _ |- _ ] => destruct H
     end; subst.
+    destruct r_o, psHeap; simpl in *.
     rewrite H1, H2, H3, H4.
     rewrite refineEquiv_If_Then_Else_Bind.
     apply refine_If_Then_Else.
       simplify with monad laws; simpl.
       unfold poke'; simpl.
       remove_dependency; simpl.
-      rewrite H0.
       etransitivity.
         apply refine_under_bind; intros.
         refine pick val {| ps'Heap   := fst a
@@ -93,7 +308,7 @@ Proof.
           simplify with monad laws.
           finish honing.
         intuition.
-      simpl.
+      rewrite H0.
       finish honing.
     rewrite refineEquiv_If_Then_Else_Bind.
     subst H.
@@ -129,7 +344,6 @@ Proof.
       simpl; remove_dependency.
       do 3 setoid_rewrite refine_bind_dep_ignore.
       unfold ByteStringHeap.buffer_cons_obligation_2.
-      rewrite H0.
       etransitivity.
         apply refine_under_bind; intros.
         etransitivity.
@@ -149,6 +363,8 @@ Proof.
             simpl; finish honing.
           simpl; finish honing.
         simpl; finish honing.
+      unfold alloc; simpl.
+      rewrite H0.
       simpl; finish honing.
     unfold allocate_buffer, alloc', poke'.
     simplify with monad laws; simpl.
@@ -156,7 +372,6 @@ Proof.
     setoid_rewrite refine_bind_dep_ret.
     autorewrite with monad laws; simpl.
     remove_dependency.
-    rewrite H0.
     unfold ByteStringHeap.buffer_cons_obligation_3.
     etransitivity.
       apply refine_under_bind; intros.
@@ -170,7 +385,8 @@ Proof.
         rewrite HeqM.
         finish honing.
       intuition.
-    simpl.
+    unfold alloc; simpl.
+    rewrite H0.
     finish honing.
   }
   {
@@ -222,25 +438,7 @@ Record CPS := {
 Variable cheap : ComputationalADT.cRep (projT1 HeapImpl).
 Variable AbsR : Heap_AbsR (` heap) cheap.
 
-(*
-Lemma refine_pick_PS' : forall P a b c d,
-  refine {r_n0 : PS' | P (ps'Heap r_n0) /\
-                       a = ps'Buffer r_n0 /\
-                       b = ps'BufLen r_n0 /\
-                       c = ps'Offset r_n0 /\
-                       d = ps'Length r_n0}
-         (r_n' <- {r_n0 : N * M.t MemoryBlockC | P r_n0};
-          {r_n0 : PS' | r_n' = ps'Heap   r_n0 /\
-                        a = ps'Buffer r_n0 /\
-                        b = ps'BufLen r_n0 /\
-                        c = ps'Offset r_n0 /\
-                        d = ps'Length r_n0}).
-Proof.
-Admitted.
-*)
-
-Lemma ByteStringFMap :
-  { adt : _ & refineADT (projT1 ByteStringStrip) adt }.
+Lemma ByteStringFMap : { adt : _ & refineADT (projT1 ByteStringStrip) adt }.
 Proof.
   eexists.
   hone representation using
@@ -267,7 +465,25 @@ Proof.
     rewrite H1, H2, H3, H4.
     rewrite refineEquiv_If_Then_Else_Bind.
     apply refine_If_Then_Else.
+      erewrite Heap_refine_poke; eauto.
+      simplify with monad laws; simpl.
+      remember (M.mapi _ _) as M.
+      refine pick val {| cpsHeap   := (fst (cpsHeap r_n), M)
+                       ; cpsBuffer := cpsBuffer r_n
+                       ; cpsBufLen := cpsBufLen r_n
+                       ; cpsOffset := cpsOffset r_n - 1
+                       ; cpsLength := cpsLength r_n + 1 |}.
+        simplify with monad laws; simpl.
+        rewrite HeqM; clear HeqM.
+        finish honing.
+      rewrite HeqM; clear HeqM.
+      intuition; simpl.
+      destruct H0.
+      apply of_map_Heap_AbsR.
       admit.
+    split; simpl.
+      split; intros.
+      apply Map_Map_AbsR.
     rewrite refineEquiv_If_Then_Else_Bind.
     subst H.
     apply refine_If_Then_Else.
@@ -298,6 +514,7 @@ Proof.
   }
   apply reflexivityT.
 Admitted.
+*)
 
 End Refined.
 
